prove that memory size is always a multiple of 8

src/ListMemory.v
@@ -10,6 +10,38 @@ Require Import riscv.Memory.
 Require Import riscv.util.Tactics.
 Require riscv.ListMemoryNatAddr.
 
+Definition align(alignment: nat)(n: nat): nat := alignment * (n / alignment).
+
+Lemma align_lt: forall a n,
+    a <> 0 ->
+    align a n <= n.
+Proof.
+  intros. unfold align.
+  apply Nat.mul_div_le.
+  assumption.
+Qed.
+
+Lemma align8_lt: forall n, align 8 n <= n.
+Proof.
+  intros. apply align_lt. congruence.
+Qed.
+
+Lemma align_eq: forall a n,
+    a <> 0 ->
+    n mod a = 0 ->
+    align a n = n.
+Proof.
+  intros. unfold align. symmetry. apply Nat.div_exact; assumption.
+Qed.
+
+Lemma align8_eq: forall n,
+    n mod 8 = 0 ->
+    align 8 n = n.
+Proof.
+  intros. apply align_eq; congruence.
+Qed.
+  
+
 (* bitwidth w is ignored on RHS, but we still want to carry it in the type *)
 Definition mem(w: nat) := ListMemoryNatAddr.mem.
 
@@ -17,7 +49,7 @@ Section Memory.
 
   Context {w: nat}. (* bit width of memory addresses *)
 
-  Definition mem_size(m: mem w): nat := min (pow2 w) (ListMemoryNatAddr.mem_size m).
+  Definition mem_size(m: mem w): nat := align 8 (min (pow2 w) (ListMemoryNatAddr.mem_size m)).
 
   Definition read_byte(m: mem w)(a: word w): word 8 :=
     ListMemoryNatAddr.read_byte m (wordToNat a).
@@ -43,11 +75,24 @@ Section Memory.
   Definition write_double(m: mem w)(a: word w)(v: word 64): mem w :=
     ListMemoryNatAddr.write_double m (wordToNat a) v.
 
-  Definition const_mem(default: word 8)(max_addr: nat): mem w :=
-    ListMemoryNatAddr.const_mem default (S max_addr).
+  Definition const_mem(default: word 8)(size: nat): mem w :=
+    ListMemoryNatAddr.const_mem default size.
 
   Definition zero_mem: nat -> mem w := const_mem $0.
 
+  (* Since mem_size is a bit fancy, we better prove that it's possible to create memory of any
+     desired size (as long as it's a multiple of 8 and not bigger than the biggest address) *)
+  Lemma const_mem_mem_size: forall size default,
+      size mod 8 = 0 ->
+      size <= pow2 w ->
+      mem_size (const_mem default size) = size.
+  Proof.
+    intros. unfold mem_size. rewrite ListMemoryNatAddr.const_mem_mem_size.
+    replace (Init.Nat.min (pow2 w) size) with size by momega.
+    apply align8_eq.
+    assumption.
+  Qed.
+            
 End Memory.
 
 Lemma wordToNat_wplus'': forall sz (a: word sz) (b: nat),
@@ -57,18 +102,24 @@ Proof.
   rewrite wordToNat_natToWord_2; omega.
 Qed.
 
+Ltac pose_align8_lt :=
+  repeat match goal with
+         | _: context [align 8 ?x] |- _=> unique pose proof (align8_lt x)
+         | |- context [align 8 ?x]     => unique pose proof (align8_lt x)
+         end.
+
 Local Ltac wrap L :=
   intros;
   repeat match goal with
          | H: valid_addr _ _ _ |- _ => destruct H
          end;
   unfold mem_size, ListMemoryNatAddr.mem_size in *;
-  first [f_equal; apply L | apply L];
+  first [do 2 f_equal; apply L | apply L];
   unfold ListMemoryNatAddr.mem_size;
+  pose_align8_lt;
   try apply wordToNat_neq1;
   (congruence || momega || idtac).    
 
-Definition TODO{T: Type}: T. Admitted.
 
 Instance mem_is_Memory(w: nat): Memory (mem w) w := {|
   memSize     := mem_size;
@@ -81,8 +132,8 @@ Instance mem_is_Memory(w: nat): Memory (mem w) w := {|
   storeWord   := write_word;
   storeDouble := write_double;
 |}.
-- intros. unfold mem_size. momega.
-- apply TODO.
+- intros. unfold mem_size. pose_align8_lt. momega.
+- intros. unfold mem_size, align. rewrite Nat.mul_comm. apply Nat.mod_mul. congruence.
 - wrap ListMemoryNatAddr.write_read_byte_eq.
 - wrap ListMemoryNatAddr.write_read_byte_ne.
 - wrap ListMemoryNatAddr.write_byte_preserves_mem_size.
@@ -96,9 +147,9 @@ Instance mem_is_Memory(w: nat): Memory (mem w) w := {|
 - wrap ListMemoryNatAddr.write_read_double_ne.
 - wrap ListMemoryNatAddr.write_double_preserves_mem_size.
 - unfold read_byte.
-  intros. unfold valid_addr, mem_size in *. rewrite wordToNat_wplus'' by momega. reflexivity.
+  intros. unfold valid_addr, mem_size in *. pose_align8_lt. rewrite wordToNat_wplus'' by momega. reflexivity.
 - unfold read_half.
-  intros. unfold valid_addr, mem_size in *. rewrite wordToNat_wplus'' by momega. reflexivity.
+  intros. unfold valid_addr, mem_size in *. pose_align8_lt. rewrite wordToNat_wplus'' by momega. reflexivity.
 - unfold read_word.
-  intros. unfold valid_addr, mem_size in *. rewrite wordToNat_wplus'' by momega. reflexivity.
+  intros. unfold valid_addr, mem_size in *. pose_align8_lt. rewrite wordToNat_wplus'' by momega. reflexivity.
 Defined.
